Replaced "is_nat" and "is_int" by "Nats" and "Ints", respectively

Fun_Conv.thy
@@ -19,18 +19,18 @@ definition to_int_fun :: "('a \<Rightarrow> 'b::floor_ceiling) \<Rightarrow> 'a 
 definition of_rat_fun :: "('a \<Rightarrow> rat) \<Rightarrow> 'a \<Rightarrow> 'b::field_char_0" where "of_rat_fun f = of_rat \<circ> f"
 
 definition to_nat_fun :: "('a \<Rightarrow> 'b::floor_ceiling) \<Rightarrow> 'a \<Rightarrow> nat" where "to_nat_fun f = to_nat \<circ> f"
-  
-definition is_int :: "'b::{floor_ceiling} \<Rightarrow> bool" where
-  "is_int x = (of_int (floor x) = x)"
 
-definition is_int_fun :: "('a \<Rightarrow> 'b::floor_ceiling) \<Rightarrow> bool" where
-  "is_int_fun f = (\<forall>x. is_int (f x))"
+definition is_int_fun :: "('a \<Rightarrow> 'b::ring_1) \<Rightarrow> bool" where
+  "is_int_fun f \<longleftrightarrow> range f \<subseteq> \<int>"
 
-definition is_nat :: "'b::floor_ceiling \<Rightarrow> bool" where
-  "is_nat x = (of_nat (to_nat x) = x)"
+definition is_nat_fun :: "('a \<Rightarrow> 'b::semiring_1) \<Rightarrow> bool" where
+  "is_nat_fun f \<longleftrightarrow> range f \<subseteq> \<nat>"
 
-definition is_nat_fun :: "('a \<Rightarrow> 'b::floor_ceiling) \<Rightarrow> bool" where
-  "is_nat_fun f = (\<forall>x. is_nat (f x))"
+lemma Ints_alt: "x \<in> \<int> \<longleftrightarrow> of_int \<lfloor>x\<rfloor> = x"
+  by (auto elim: Ints_cases)
+
+lemma Nats_alt: "x \<in> \<nat> \<longleftrightarrow> of_nat (to_nat x) = x"
+  by (auto simp: to_nat_def Nats_def dest: sym)
   
 lemma to_nat_comp_of_nat: "to_nat \<circ> of_nat = id"
   by (auto simp: to_nat_def)
@@ -59,13 +59,32 @@ lemma nat_comp_of_nat_fun: "nat \<circ> (of_nat_fun f) = f"
 lemma to_nat_comp_of_nat_fun: "to_nat \<circ> (of_nat_fun f) = f"
   by (simp add: comp_def of_nat_fun_def to_nat_of_nat)
 
+lemma is_int_fun_alt: "is_int_fun f \<longleftrightarrow> (\<forall>x. f x \<in> \<int>)"
+  by (auto simp: is_int_fun_def)
+
+lemma is_int_funI: "(\<And>x. f x \<in> \<int>) \<Longrightarrow> is_int_fun f"
+  by (simp add: is_int_fun_alt)
+
+lemma is_int_funD: "is_int_fun f \<Longrightarrow> f x \<in> \<int>"
+  by (simp add: is_int_fun_alt)
+
+lemma is_nat_fun_alt: "is_nat_fun f \<longleftrightarrow> (\<forall>x. f x \<in> \<nat>)"
+  by (auto simp: is_nat_fun_def)
+
+lemma is_nat_funI: "(\<And>x. f x \<in> \<nat>) \<Longrightarrow> is_nat_fun f"
+  by (simp add: is_nat_fun_alt)
+
+lemma is_nat_funD: "is_nat_fun f \<Longrightarrow> f x \<in> \<nat>"
+  by (simp add: is_nat_fun_alt)
+
 lemma of_int_fun_comp_to_int_fun:
   assumes "is_int_fun f"
   shows "of_int_fun (to_int_fun f) = f"
   unfolding of_int_fun_def to_int_fun_def comp_def
 proof
   fix x
-  from assms show "of_int \<lfloor>f x\<rfloor> = f x" unfolding is_int_fun_def is_int_def ..
+  from assms have "f x \<in> \<int>" by (rule is_int_funD)
+  thus "of_int \<lfloor>f x\<rfloor> = f x" by (simp only: Ints_alt)
 qed
 
 lemma of_int_fun_comp_of_nat_fun: "of_int_fun (of_nat_fun f) = of_nat_fun f"
@@ -86,7 +105,8 @@ lemma of_nat_fun_comp_to_nat_fun:
   unfolding of_nat_fun_def to_nat_fun_def comp_def
 proof
   fix x
-  from assms show "of_nat (to_nat (f x)) = f x" unfolding is_nat_fun_def is_nat_def ..
+  from assms have "f x \<in> \<nat>" by (rule is_nat_funD)
+  thus "of_nat (to_nat (f x)) = f x" by (simp only: Nats_alt)
 qed
 
 lemma of_nat_fun_comp_to_nat_fun_eq_to_int_fun:
@@ -95,64 +115,51 @@ lemma of_nat_fun_comp_to_nat_fun_eq_to_int_fun:
   unfolding of_nat_fun_def to_nat_fun_def to_nat_def to_int_fun_def comp_def
 proof
   fix x
-  from assms have "is_nat (f x)" unfolding is_nat_fun_def ..
-  hence "of_nat (nat \<lfloor>f x\<rfloor>) = f x" unfolding is_nat_def to_nat_def comp_def .
+  from assms have "f x \<in> \<nat>" by (rule is_nat_funD)
+  hence "of_nat (nat \<lfloor>f x\<rfloor>) = f x" by (simp only: Nats_alt to_nat_def comp_def)
   hence "\<lfloor>(of_nat (nat \<lfloor>f x\<rfloor>))::'b\<rfloor> = \<lfloor>f x\<rfloor>" by simp
   thus "int (nat \<lfloor>f x\<rfloor>) = \<lfloor>f x\<rfloor>" by simp
 qed
   
-lemma nat_is_int: "is_nat x \<Longrightarrow> is_int x"
-  unfolding is_nat_def is_int_def by (metis floor_of_nat of_int_of_nat_eq)
+lemma Nats_imp_Ints: "x \<in> \<nat> \<Longrightarrow> x \<in> \<int>"
+  using Nats_subset_Ints ..
 
 lemma nat_fun_is_int_fun: "is_nat_fun f \<Longrightarrow> is_int_fun f"
-  unfolding is_nat_fun_def is_int_fun_def using nat_is_int by auto
+  unfolding is_nat_fun_def is_int_fun_def using Nats_imp_Ints by auto
 
-lemma is_nat_geq_zero: "is_nat x \<Longrightarrow> 0 \<le> x"
-  unfolding is_nat_def by (metis of_nat_0_le_iff)
+lemma Nats_ge_0: "x \<in> \<nat> \<Longrightarrow> 0 \<le> (x::_::linordered_idom)"
+  by (simp add: Nats_altdef2)
 
-lemma int_is_nat:
-  assumes "is_int x" and "0 \<le> x"
-  shows "is_nat x"
-proof -
-  from assms(1) have "x = of_int \<lfloor>x\<rfloor>" unfolding is_int_def by auto
-  with assms(2) show "is_nat x" unfolding is_nat_def
-    by (metis comp_def of_int_le_iff of_int_0 of_nat_nat to_nat_def)
-qed
+lemma Ints_imp_Nats: "x \<in> \<int> \<Longrightarrow> 0 \<le> (x::_::linordered_idom) \<Longrightarrow> x \<in> \<nat>"
+  by (simp add: Nats_altdef2) 
 
 lemma int_fun_is_nat_fun:
-  assumes "is_int_fun f" and "\<And>x. 0 \<le> f x"
+  assumes "is_int_fun f" and "\<And>x. (0::_::linordered_idom) \<le> f x"
   shows "is_nat_fun f"
-  unfolding is_nat_fun_def
-proof
+proof (rule is_nat_funI)
   fix x
-  from assms(1) have "is_int (f x)" unfolding is_int_fun_def ..
+  from assms(1) have "f x \<in> \<int>" by (rule is_int_funD)
   moreover from assms(2) have "0 \<le> f x" .
-  ultimately show "is_nat (f x)" by (rule int_is_nat)
+  ultimately show "f x \<in> \<nat>" by (rule Ints_imp_Nats)
 qed
 
 lemma int_fun_is_nat_funI:
-  assumes "is_int_fun f" and "is_nat_fun g" and "g \<le> (f::_ \<Rightarrow> _::preorder)"
+  assumes "is_int_fun f" and "is_nat_fun g" and "g \<le> (f::_ \<Rightarrow> _::linordered_idom)"
   shows "is_nat_fun f"
   using assms(1)
 proof (rule int_fun_is_nat_fun)
   fix x
-  from assms(2) have "is_nat (g x)" by (simp only: is_nat_fun_def)
-  hence "0 \<le> g x" by (rule is_nat_geq_zero)
+  from assms(2) have "g x \<in> \<nat>" by (rule is_nat_funD)
+  hence "0 \<le> g x" by (rule Nats_ge_0)
   also from assms(3) have "\<dots> \<le> f x" by (rule le_funD)
   finally show "0 \<le> (f x)" .
 qed
 
-lemma of_nat_is_nat: "is_nat (of_nat n)"
-  unfolding is_nat_def to_nat_def by simp
-    
-lemma of_int_is_int: "is_int (of_int a)"
-  unfolding is_int_def by simp
-
 lemma of_nat_fun_is_nat_fun: "is_nat_fun (of_nat_fun f)"
-  unfolding is_nat_fun_def of_nat_fun_def comp_def by (simp add: of_nat_is_nat)
+  by (rule is_nat_funI) (simp add: of_nat_fun_def)
 
 lemma of_int_fun_is_int_fun: "is_int_fun (of_int_fun f)"
-  unfolding is_int_fun_def of_int_fun_def comp_def by (simp add: of_int_is_int)
+  by (rule is_int_funI) (simp add: is_int_fun_def of_int_fun_def)
 
 lemma max_of_nat:
   "(\<And>m n::nat. of_nat m \<le> ((of_nat n)::'b::{semiring_1,ord}) \<longleftrightarrow> m \<le> n) \<Longrightarrow>
@@ -188,8 +195,8 @@ lemma less_of_int_fun: "of_int_fun f < ((of_int_fun g)::'a \<Rightarrow> ('b::li
 lemma to_nat_mono: "x \<le> y \<Longrightarrow> to_nat x \<le> to_nat y"
   by (auto simp: to_nat_def dest: floor_mono)
 
-lemma of_nat_to_nat_ge: "is_int x \<Longrightarrow> x \<le> of_nat (to_nat x)"
-  by (metis int_is_nat is_nat_def linear of_nat_0_le_iff order_trans)
+lemma of_nat_to_nat_ge: "x \<in> \<int> \<Longrightarrow> x \<le> of_nat (to_nat (x::_::floor_ceiling))"
+  by (metis Ints_imp_Nats Nats_alt linear of_nat_0_le_iff order_trans)
 
 lemma to_nat_fun_mono: "f \<le> g \<Longrightarrow> to_nat_fun f \<le> to_nat_fun g"
   by (auto simp: to_nat_fun_def le_fun_def dest: to_nat_mono)
@@ -197,24 +204,8 @@ lemma to_nat_fun_mono: "f \<le> g \<Longrightarrow> to_nat_fun f \<le> to_nat_fu
 lemma to_int_fun_mono: "f \<le> g \<Longrightarrow> to_int_fun f \<le> to_int_fun g"
   by (auto simp: to_int_fun_def comp_def le_fun_def dest: floor_mono)
 
-lemma is_int_less_iff: "is_int a \<Longrightarrow> is_int b \<Longrightarrow> a < b \<longleftrightarrow> a + 1 \<le> b"
-  by (metis floor_unique is_int_def le_less less_add_one less_trans not_less)
-
-subsection \<open>Closure Properties of @{const is_nat} and @{const is_int}\<close>
-  
-subsubsection \<open>0 and 1\<close>
-
-lemma zero_is_nat: "is_nat 0"
-  by (metis of_nat_0 of_nat_is_nat)
-
-lemma one_is_nat: "is_nat 1"
-  by (metis of_nat_1 of_nat_is_nat)
-
-lemma zero_is_int: "is_int 0"
-  using zero_is_nat by (rule nat_is_int)
-
-lemma one_is_int: "is_int 1"
-  using one_is_nat by (rule nat_is_int)
+lemma is_int_less_iff: "a \<in> \<int> \<Longrightarrow> b \<in> \<int> \<Longrightarrow> a < b \<longleftrightarrow> a + 1 \<le> (b::_::floor_ceiling)"
+  by (metis floor_unique Ints_alt le_less less_add_one less_trans not_less)
 
 lemma to_nat_zero [simp]: "to_nat 0 = 0"
   by (simp add: to_nat_def)
@@ -222,44 +213,25 @@ lemma to_nat_zero [simp]: "to_nat 0 = 0"
 lemma to_nat_one [simp]: "to_nat 1 = 1"
   by (simp add: to_nat_def)
 
+subsection \<open>Closure Properties of @{const Nats} and @{const Ints}\<close>
+
 subsubsection \<open>@{const plus} and @{const minus}\<close>
 
-lemma plus_is_nat:
-  assumes "is_nat x" and "is_nat y"
-  shows "is_nat (x + y)"
-  using assms unfolding is_nat_def
-proof -
-  assume a1: "of_nat (to_nat x) = x"
-  assume a2: "of_nat (to_nat y) = y"
-  have f3: "to_nat (x + y) = nat \<lfloor>x + y\<rfloor>" by (metis comp_apply to_nat_def)
-  have "x + y = of_nat (to_nat x) + of_nat (to_nat y)" using a2 a1 by presburger
-  thus "of_nat (to_nat (x + y)) = x + y" using f3 by simp
-qed
+lemma Nats_minus: "x \<in> \<int> \<Longrightarrow> y \<in> \<int> \<Longrightarrow> x - y \<in> \<nat> \<longleftrightarrow> y \<le> (x::_::floor_ceiling)"
+  unfolding Nats_alt Ints_alt
+  by (metis diff_ge_0_iff_ge Ints_imp_Nats Nats_alt of_int_diff Ints_of_int of_nat_0_le_iff)
 
-lemma minus_is_nat: "is_int x \<Longrightarrow> is_int y \<Longrightarrow> is_nat (x - y) \<longleftrightarrow> y \<le> x"
-  unfolding is_nat_def is_int_def
-  by (metis diff_ge_0_iff_ge int_is_nat is_nat_def of_int_diff of_int_is_int of_nat_0_le_iff)
+lemma Nats_sum: "(\<And>a. a \<in> A \<Longrightarrow> f a \<in> \<nat>) \<Longrightarrow> sum f A \<in> \<nat>"
+  by (induct A rule: infinite_finite_induct) (auto intro: Nats_0 Nats_add)
 
-lemma plus_is_int: "is_int x \<Longrightarrow> is_int y \<Longrightarrow> is_int (x + y)"
-  by (metis is_int_def of_int_floor_cancel of_int_add)
+lemma Ints_sum: "(\<And>a. a \<in> A \<Longrightarrow> f a \<in> \<int>) \<Longrightarrow> sum f A \<in> \<int>"
+  by (induct A rule: infinite_finite_induct) (auto intro: Ints_0 Ints_add)
 
-lemma minus_is_int:"is_int x \<Longrightarrow> is_int y \<Longrightarrow> is_int (x - y)"
-  by (metis is_int_def of_int_floor_cancel of_int_diff)
-
-lemma uminus_is_int: "is_int x \<Longrightarrow> is_int (- x)"
-  by (metis is_int_def of_int_floor_cancel of_int_minus)
-
-lemma sum_is_nat: "(\<And>a. a \<in> A \<Longrightarrow> is_nat (f a)) \<Longrightarrow> is_nat (sum f A)"
-  by (induct A rule: infinite_finite_induct) (auto intro: zero_is_nat plus_is_nat)
-
-lemma sum_is_int: "(\<And>a. a \<in> A \<Longrightarrow> is_int (f a)) \<Longrightarrow> is_int (sum f A)"
-  by (induct A rule: infinite_finite_induct) (auto intro: zero_is_int plus_is_int)
-
-lemma to_nat_plus_le: "is_int a \<Longrightarrow> is_int b \<Longrightarrow> to_nat (a + b) \<le> to_nat a + to_nat b"
-  by (metis (full_types) add_le_same_cancel1 add_le_same_cancel2 int_is_nat is_nat_def linear
+lemma to_nat_plus_le: "a \<in> \<int> \<Longrightarrow> b \<in> \<int> \<Longrightarrow> to_nat (a + b) \<le> to_nat a + to_nat (b::_::linordered_idom)"
+  by (metis (full_types) add_le_same_cancel1 add_le_same_cancel2 Ints_imp_Nats Nats_alt linear
       of_nat_add to_nat_mono to_nat_of_nat trans_le_add1 trans_le_add2)
 
-lemma to_nat_sum_le: "(\<And>a. a \<in> A \<Longrightarrow> is_int (f a)) \<Longrightarrow> to_nat (sum f A) \<le> (\<Sum>a\<in>A. to_nat (f a))"
+lemma to_nat_sum_le: "(\<And>a. a \<in> A \<Longrightarrow> f a \<in> \<int>) \<Longrightarrow> to_nat (sum f A) \<le> (\<Sum>a\<in>A. to_nat (f a))"
 proof (induct A rule: infinite_finite_induct)
   case (infinite A)
   thus ?case by simp
@@ -268,9 +240,9 @@ next
   thus ?case by simp
 next
   case (insert a A)
-  have rl: "\<And>x. x \<in> A \<Longrightarrow> is_int (f x)" by (auto intro: insert.prems)
-  hence "is_int (sum f A)" by (rule sum_is_int)
-  have "is_int (f a)" by (rule insert.prems) simp
+  have rl: "\<And>x. x \<in> A \<Longrightarrow> f x \<in> \<int>" by (auto intro: insert.prems)
+  hence "sum f A \<in> \<int>" by (rule Ints_sum)
+  have "f a \<in> \<int>" by (rule insert.prems) simp
   from insert.hyps(1, 2) have "to_nat (sum f (insert a A)) = to_nat (f a + sum f A)" by simp
   also have "\<dots> \<le> to_nat (f a) + to_nat (sum f A)" by (rule to_nat_plus_le) fact+
   also have "\<dots> \<le> to_nat (f a) + (\<Sum>x\<in>A. to_nat (f x))" by (intro add_left_mono insert.hyps rl)
@@ -280,41 +252,32 @@ qed
 
 subsubsection \<open>@{const times}\<close>
 
-lemma times_is_nat: "is_nat x \<Longrightarrow> is_nat y \<Longrightarrow> is_nat (x * y)"
-  by (metis is_nat_def of_nat_is_nat of_nat_mult)
+lemma Nats_prod: "(\<And>a. a \<in> A \<Longrightarrow> f a \<in> \<nat>) \<Longrightarrow> prod f A \<in> \<nat>"
+  by (induct A rule: infinite_finite_induct) (auto intro: Nats_1 Nats_mult)
 
-lemma times_is_int: "is_int x \<Longrightarrow> is_int y \<Longrightarrow> is_int (x * y)"
-  by (metis is_int_def of_int_floor_cancel of_int_mult)
-
-lemma prod_is_nat: "(\<And>a. a \<in> A \<Longrightarrow> is_nat (f a)) \<Longrightarrow> is_nat (prod f A)"
-  by (induct A rule: infinite_finite_induct) (auto intro: one_is_nat times_is_nat)
-
-lemma prod_is_int: "(\<And>a. a \<in> A \<Longrightarrow> is_int (f a)) \<Longrightarrow> is_int (prod f A)"
-  by (induct A rule: infinite_finite_induct) (auto intro: one_is_int times_is_int)
+lemma Ints_prod: "(\<And>a. a \<in> A \<Longrightarrow> f a \<in> \<int>) \<Longrightarrow> prod f A \<in> \<int>"
+  by (induct A rule: infinite_finite_induct) (auto intro: Ints_1 Ints_mult)
 
 subsubsection \<open>@{const min} and @{const max}\<close>
 
-lemma min_is_nat:"is_nat x \<Longrightarrow> is_nat y \<Longrightarrow> is_nat (min x y)"
+lemma Nats_min: "x \<in> \<nat> \<Longrightarrow> y \<in> \<nat> \<Longrightarrow> min x y \<in> \<nat>"
   by (simp add: min_def)
 
-lemma max_is_nat: "is_nat x \<Longrightarrow> is_nat y \<Longrightarrow> is_nat (max x y)"
+lemma Nats_max: "x \<in> \<nat> \<Longrightarrow> y \<in> \<nat> \<Longrightarrow> max x y \<in> \<nat>"
   by (simp add: max_def)
 
-lemma max_is_nat': "is_nat x \<Longrightarrow> is_int y \<Longrightarrow> is_nat (max x y)"
-  by (metis int_is_nat is_nat_geq_zero le_max_iff_disj max_def)
+lemma Nats_max': "x \<in> \<nat> \<Longrightarrow> y \<in> \<int> \<Longrightarrow> max x (y::_::linordered_idom) \<in> \<nat>"
+  by (metis Ints_imp_Nats Nats_ge_0 le_max_iff_disj max_def)
 
-lemma min_is_int: "is_int x \<Longrightarrow> is_int y \<Longrightarrow> is_int (min x y)"
+lemma Ints_min: "x \<in> \<int> \<Longrightarrow> y \<in> \<int> \<Longrightarrow> min x y \<in> \<int>"
   by (simp add: min_def)
 
-lemma max_is_int: "is_int x \<Longrightarrow> is_int y \<Longrightarrow> is_int (max x y)"
+lemma Ints_max: "x \<in> \<int> \<Longrightarrow> y \<in> \<int> \<Longrightarrow> max x y \<in> \<int>"
   by (simp add: max_def)
 
 subsubsection \<open>@{const abs}\<close>
 
-lemma abs_is_int: "is_int x \<Longrightarrow> is_int \<bar>x\<bar>"
-  by (metis abs_abs abs_eq_iff uminus_is_int)
-
-lemma abs_is_nat: "is_int x \<Longrightarrow> is_nat \<bar>x\<bar>"
-  by (intro int_is_nat abs_is_int abs_ge_zero)
+lemma Nats_abs: "x \<in> \<int> \<Longrightarrow> \<bar>x::_::linordered_idom\<bar> \<in> \<nat>"
+  by (intro Ints_imp_Nats Ints_abs abs_ge_zero)
   
 end (* theory *)
